Remove Eq_list

Coq/src/Eq.v
@@ -7,55 +7,12 @@ Require Import Equivalence.
 
 Set Implicit Arguments.
 
-Section Eq_list.
+Section Eq_Prog.
   Variable A : Type.
-  Variable eq_A : A -> A -> Prop.
-  
-  Variable eq_A_refl  : Reflexive eq_A.
-  Variable eq_A_symm  : Symmetric eq_A.
-  Variable eq_A_trans : Transitive eq_A.
-  
-  Inductive Eq_list : list A -> list A -> Prop :=
-  | eq_nil  : Eq_list nil nil
-  | eq_cons : forall x y xs ys,
-      eq_A x y ->
-    Eq_list xs ys ->
-    Eq_list (cons x xs) (cons y ys).
-  
-  Lemma eq_list_refl : Reflexive Eq_list.
-  Proof.
-    intros xs.
-    induction xs as [ | y ys].
-    - constructor.
-    - constructor.
-      + reflexivity.
-      + assumption.
-  Qed.
+  Variable NF__A : Normalform A A.
 
-  Lemma eq_list_symm : Symmetric Eq_list.
-  Proof.
-    intros xs ys H.
-    induction H; constructor.
-    - symmetry. assumption.
-    - assumption.
-  Qed.
+  Definition Eq_Prog (p1 p2 : Prog A) := handle p1 = handle p2.
 
-  Lemma eq_list_trans : Transitive Eq_list.
-  Proof with auto; try constructor; auto.
-    intros xs.
-    induction xs; intros ys zs H1 H2; inversion H1; subst; inversion H2; subst...
-    - etransitivity. apply H3. assumption.
-    - apply IHxs with (y := ys0); assumption.
-  Qed.
-
-  Global Instance eq_list_Reflexive : Reflexive Eq_list := eq_list_refl.
-  Global Instance eq_list_Symmetric : Symmetric Eq_list := eq_list_symm.
-  Global Instance eq_list_Transitive : Transitive Eq_list := eq_list_trans.
-
-  Definition Eq_Prog `{Normalform A A} (p1 p2 : Prog A) :=
-    Eq_list (handle p1) (handle p2).
-
-  Variable nf__A : (Normalform A A).
   Lemma eq_Prog_refl : Reflexive Eq_Prog.
   Proof. 
     intros p.
@@ -66,8 +23,7 @@ Section Eq_list.
   Lemma eq_Prog_symm : Symmetric Eq_Prog.
   Proof.
     intros p1 p2 H.
-    unfold Eq_Prog.
-    unfold Eq_Prog in H.
+    unfold Eq_Prog in *.
     symmetry.
     assumption.
   Qed.
@@ -75,15 +31,13 @@ Section Eq_list.
   Lemma eq_Prog_trans : Transitive Eq_Prog.
   Proof.
     intros p1 p2 p3 H1 H2.
-    unfold Eq_Prog.
-    unfold Eq_Prog in H1, H2.
+    unfold Eq_Prog in *.
     etransitivity.
     apply H1.
     assumption.
   Qed.
 
-  Global Instance eq_Prog_Reflexive : Reflexive Eq_Prog := eq_Prog_refl.
-  Global Instance eq_Prog_Symmetric : Symmetric Eq_Prog := eq_Prog_symm.
+  Global Instance eq_Prog_Reflexive  : Reflexive Eq_Prog  := eq_Prog_refl.
+  Global Instance eq_Prog_Symmetric  : Symmetric Eq_Prog  := eq_Prog_symm.
   Global Instance eq_Prog_Transitive : Transitive Eq_Prog := eq_Prog_trans.
-
-End Eq_list.
+End Eq_Prog.
